James C - got proof of concept stack compilation going

StackToAssembly.thy
@@ -3,63 +3,60 @@ imports StackLanguage AssemblyLanguage Iterate
 begin
 
 primrec instruction_conv :: "stack_instruction \<Rightarrow> assembly list" where
-  "instruction_conv Add = [AAssm 0, CAssm {A} (Reg M), CAssm {D} (Reg M), AAssm 0, CAssm {A, M} (Decr M), CAssm {M} DPlusM]"
-| "instruction_conv Sub = [AAssm 0, CAssm {A} (Reg M), CAssm {D} (Reg M), AAssm 0, CAssm {A, M} (Decr M), CAssm {M} MMinusD]"
-| "instruction_conv Neg = [AAssm 0, CAssm {A} (Reg M), CAssm {M} (NegR M)]"
+  "instruction_conv Add = [CAssm {A} (Reg M), CAssm {D} (Reg M), AAssm 0, CAssm {A, M} (Decr M), CAssm {M} DPlusM, AAssm 0]"
+| "instruction_conv Sub = [CAssm {A} (Reg M), CAssm {D} (Reg M), AAssm 0, CAssm {A, M} (Decr M), CAssm {M} MMinusD, AAssm 0]"
+| "instruction_conv Neg = [CAssm {A} (Reg M), CAssm {M} (NegR M), AAssm 0]"
 | "instruction_conv Eq = undefined"
 | "instruction_conv Gt = undefined"
 | "instruction_conv Lt = undefined"
-| "instruction_conv And = [AAssm 0, CAssm {A} (Reg M), CAssm {D} (Reg M), AAssm 0, CAssm {A, M} (Decr M), CAssm {M} DAndM]"
-| "instruction_conv Or = [AAssm 0, CAssm {A} (Reg M), CAssm {D} (Reg M), AAssm 0, CAssm {A, M} (Decr M), CAssm {M} DOrM]"
-| "instruction_conv Not = [AAssm 0, CAssm {A} (Reg M), CAssm {D} (NotR M)]"
+| "instruction_conv And = [CAssm {A} (Reg M), CAssm {D} (Reg M), AAssm 0, CAssm {A, M} (Decr M), CAssm {M} DAndM, AAssm 0]"
+| "instruction_conv Or = [CAssm {A} (Reg M), CAssm {D} (Reg M), AAssm 0, CAssm {A, M} (Decr M), CAssm {M} DOrM, AAssm 0]"
+| "instruction_conv Not = [CAssm {A} (Reg M), CAssm {D} (NotR M), AAssm 0]"
 
 definition program_convert :: "stack_program \<Rightarrow> assembly_program" where
   "program_convert \<Pi> = map_option concat o map_option (map instruction_conv) o \<Pi>"
 
 primrec stack_to_mem :: "int list \<Rightarrow> (int \<Rightarrow> int) \<Rightarrow> int \<Rightarrow> int" where
-  "stack_to_mem [] \<mu> k = \<mu> k"
-| "stack_to_mem (i # is) \<mu> k = (if k > 0 \<and> nat k = Suc (length is) then i else stack_to_mem is \<mu> k)" 
+  "stack_to_mem [] \<mu> k = (if k = 0 then 0 else \<mu> k)"
+| "stack_to_mem (i # is) \<mu> k = (
+    if k = 0 then 1 + int (length is) 
+    else if k > 0 \<and> k = 1 + int (length is) then i 
+    else stack_to_mem is \<mu> k)" 
 
 primrec state_convert :: "stack_state \<Rightarrow> assembly_state set" where
-  "state_convert (\<sigma>, \<pi>) = {((stack_to_mem \<sigma> \<mu>)(0 := int (length \<sigma>)), None, d, concat (map instruction_conv \<pi>)) | d \<mu>. True }"
+  "state_convert (\<sigma>, \<pi>) = {(stack_to_mem \<sigma> \<mu>, Some 0, d, concat (map instruction_conv \<pi>)) | d \<mu>. True }"
 
 (* conversion correctness *)
 
 lemma [simp]: "dom (program_convert \<Pi>) = dom \<Pi>"
   by (auto simp add: program_convert_def)
 
+lemma [simp]: "(stack_to_mem (i1 # \<sigma>) \<mu>)(1 + int (length \<sigma>) := i2) = stack_to_mem (i2 # \<sigma>) \<mu>"
+  by auto
+
 lemma eval_stack_conv [simp]: "eval_stack \<Pi> \<Sigma>\<^sub>S = Some \<Sigma>\<^sub>S' \<Longrightarrow> \<Sigma>\<^sub>A \<in> state_convert \<Sigma>\<^sub>S \<Longrightarrow> 
     \<exists>\<Sigma>\<^sub>A'. \<Sigma>\<^sub>A' \<in> state_convert \<Sigma>\<^sub>S' \<and> iterate (eval_assembly (program_convert \<Pi>)) \<Sigma>\<^sub>A \<Sigma>\<^sub>A'"
   proof (induction \<Pi> \<Sigma>\<^sub>S rule: eval_stack.induct)
   case (1 \<Pi> i1 i2 \<sigma> \<pi>)
-    then obtain d \<mu> where M: "\<Sigma>\<^sub>A = ((stack_to_mem (i1 # i2 # \<sigma>) \<mu>)(0 :=  int (Suc (Suc (length \<sigma>)))), None, d, concat (map instruction_conv (Add # \<pi>)))" by fastforce
-    from 1 have S: "\<Sigma>\<^sub>S' = ((i2 + i1) # \<sigma>, \<pi>)" by simp
-
-    let ?ev = "eval_assembly (program_convert \<Pi>)"
-    let ?\<mu>' = "(stack_to_mem (i1 # i2 # \<sigma>) \<mu>)(0 :=  int (Suc (Suc (length \<sigma>))))"
-
-    have step1: "?ev (?\<mu>', None, d, [AAssm 0, CAssm {A} (Reg M), CAssm {D} (Reg M), AAssm 0, CAssm {A, M} (Decr M), CAssm {M} DPlusM] @ concat (map instruction_conv \<pi>)) = 
-      Some (?\<mu>', Some 0, d, [CAssm {A} (Reg M), CAssm {D} (Reg M), AAssm 0, CAssm {A, M} (Decr M), CAssm {M} DPlusM] @ concat (map instruction_conv \<pi>))" by simp
-    have step2: "?ev (?\<mu>', Some 0, d, [CAssm {A} (Reg M), CAssm {D} (Reg M), AAssm 0, CAssm {A, M} (Decr M), CAssm {M} DPlusM] @ concat (map instruction_conv \<pi>)) = 
-      Some (?\<mu>', Some (?\<mu>' 0), d, [CAssm {D} (Reg M), AAssm 0, CAssm {A, M} (Decr M), CAssm {M} DPlusM] @ concat (map instruction_conv \<pi>))" by simp
-    have step3: "?ev (?\<mu>', Some (?\<mu>' 0), d, [CAssm {D} (Reg M), AAssm 0, CAssm {A, M} (Decr M), CAssm {M} DPlusM] @ concat (map instruction_conv \<pi>)) = 
-      Some (?\<mu>', Some (?\<mu>' 0), ?\<mu>' (?\<mu>' 0), [AAssm 0, CAssm {A, M} (Decr M), CAssm {M} DPlusM] @ concat (map instruction_conv \<pi>))" by simp
-    have step4: "?ev (?\<mu>', Some (?\<mu>' 0), ?\<mu>' (?\<mu>' 0), [AAssm 0, CAssm {A, M} (Decr M), CAssm {M} DPlusM] @ concat (map instruction_conv \<pi>)) = 
-      Some (?\<mu>', Some 0, ?\<mu>' (?\<mu>' 0), [CAssm {A, M} (Decr M), CAssm {M} DPlusM] @ concat (map instruction_conv \<pi>))" by simp
-    have step5: "?ev (?\<mu>', Some 0, ?\<mu>' (?\<mu>' 0), [CAssm {A, M} (Decr M), CAssm {M} DPlusM] @ concat (map instruction_conv \<pi>)) = 
-      Some (?\<mu>'(0 := ?\<mu>' 0 - 1), Some (?\<mu>' 0 - 1), ?\<mu>' (?\<mu>' 0), [CAssm {M} DPlusM] @ concat (map instruction_conv \<pi>))" by simp
-    have step6: "?ev (?\<mu>'(0 := ?\<mu>' 0 - 1), Some (?\<mu>' 0 - 1), ?\<mu>' (?\<mu>' 0), [CAssm {M} DPlusM] @ concat (map instruction_conv \<pi>)) = 
-      Some (?\<mu>'(0 := ?\<mu>' 0 - 1, ?\<mu>' 0 - 1 := ?\<mu>' (?\<mu>' 0) + ?\<mu>' (?\<mu>' 0 - 1)), Some (?\<mu>' 0 - 1), ?\<mu>' (?\<mu>' 0), concat (map instruction_conv \<pi>))" by simp
-
-
-
-    have "\<Sigma>\<^sub>A' \<in> state_convert ((i2 + i1) # \<sigma>, \<pi>) \<and> iterate ?ev (?\<mu>', None, d, [AAssm 0, CAssm {A} (Reg M), CAssm {D} (Reg M), AAssm 0, CAssm {A, M} (Decr M), CAssm {M} DPlusM] @ concat (map instruction_conv \<pi>)) \<Sigma>\<^sub>A'" by simp
-    hence "\<Sigma>\<^sub>A' \<in> state_convert ((i2 + i1) # \<sigma>, \<pi>) \<and> iterate ?ev (?\<mu>', None, d, concat (map instruction_conv (Add # \<pi>))) \<Sigma>\<^sub>A'" by simp
-    with S M show ?case by blast
+    thus ?case by simp
   next case 2
     thus ?case by simp
-  next case 3
-    thus ?case by simp
+  next case (3 \<Pi> i1 \<sigma> \<pi>)
+    let ?\<pi>' = "concat (map instruction_conv \<pi>)"
+    from 3 obtain d \<mu> where M: "\<Sigma>\<^sub>A = (stack_to_mem (i1 # \<sigma>) \<mu>, Some 0, d, 
+      [CAssm {A} (Reg M), CAssm {M} (NegR M), AAssm 0] @ ?\<pi>')" by fastforce
+    from 3 have S: "\<Sigma>\<^sub>S' = ((-i1) # \<sigma>, \<pi>)" by simp
+    let ?\<mu> = "stack_to_mem (i1 # \<sigma>) \<mu>"
+    let ?\<Sigma>\<^sub>A\<^sub>1 = "(?\<mu>, Some (?\<mu> 0), d, [CAssm {M} (NegR M), AAssm 0] @ ?\<pi>')"
+    let ?\<Sigma>\<^sub>A\<^sub>2 = "(?\<mu>(?\<mu> 0 := - ?\<mu> (?\<mu> 0)), Some (?\<mu> 0), d, [AAssm 0] @ ?\<pi>')"
+    let ?\<Sigma>\<^sub>A\<^sub>3 = "(?\<mu>(?\<mu> 0 := - ?\<mu> (?\<mu> 0)), Some 0, d, ?\<pi>')"
+    from M have step1: "eval_assembly (program_convert \<Pi>) \<Sigma>\<^sub>A = Some ?\<Sigma>\<^sub>A\<^sub>1" by simp
+    have step2: "eval_assembly (program_convert \<Pi>) ?\<Sigma>\<^sub>A\<^sub>1 = Some ?\<Sigma>\<^sub>A\<^sub>2" by simp
+    have "eval_assembly (program_convert \<Pi>) ?\<Sigma>\<^sub>A\<^sub>2 = Some ?\<Sigma>\<^sub>A\<^sub>3" by simp
+    with iter_two iter_prestep step1 step2 have X:
+      "iterate (eval_assembly (program_convert \<Pi>)) \<Sigma>\<^sub>A ?\<Sigma>\<^sub>A\<^sub>3" by fast
+    have "?\<Sigma>\<^sub>A\<^sub>3 \<in> state_convert ((-i1) # \<sigma>, \<pi>)" by auto
+    with X S M show ?case by metis
   next case 4
     thus ?case by simp
   next case 5
@@ -112,8 +109,8 @@ theorem stack_to_assembly_correct [simp]: "iterate (eval_stack \<Pi>) \<Sigma>\<
     with iter_step eval_stack_conv obtain \<Sigma>\<^sub>A'' where
         "\<Sigma>\<^sub>A'' \<in> state_convert \<Sigma>\<^sub>S'' \<and> iterate (eval_assembly (program_convert \<Pi>)) \<Sigma>\<^sub>A' \<Sigma>\<^sub>A''" 
       by blast
-    with S have "\<Sigma>\<^sub>A'' \<in> state_convert \<Sigma>\<^sub>S'' \<and> 
-      iterate (eval_assembly (program_convert \<Pi>)) \<Sigma>\<^sub>A \<Sigma>\<^sub>A''" by fastforce
+    with S have "\<Sigma>\<^sub>A'' \<in> state_convert \<Sigma>\<^sub>S'' \<and> iterate (eval_assembly (program_convert \<Pi>)) \<Sigma>\<^sub>A \<Sigma>\<^sub>A''" 
+      by fastforce
     thus ?case by blast
   qed
 
