Iterate.thy
@@ -6,14 +6,14 @@ inductive iterate :: "('a \<rightharpoonup> 'a) \<Rightarrow> 'a \<Rightarrow> '
   iter_refl [simp]: "iterate f x x"
 | iter_step [simp]: "iterate f x y \<Longrightarrow> f y = Some z \<Longrightarrow> iterate f x z"
 
-lemma [elim]: "f x = Some y \<Longrightarrow> iterate f x y"
+lemma iter_one: "f x = Some y \<Longrightarrow> iterate f x y"
   proof -
     assume "f x = Some y"
     moreover have "iterate f x x" by simp
     ultimately show ?thesis by (metis iter_step)
   qed
 
-lemma [elim]: "f x = Some y \<Longrightarrow> f y = Some z \<Longrightarrow> iterate f x z"
+lemma iter_two: "f x = Some y \<Longrightarrow> f y = Some z \<Longrightarrow> iterate f x z"
   proof -
     assume "f x = Some y"
     moreover assume "f y = Some z"
@@ -21,15 +21,15 @@ lemma [elim]: "f x = Some y \<Longrightarrow> f y = Some z \<Longrightarrow> ite
     ultimately show ?thesis by (metis iter_step)
   qed
 
-lemma [elim]: "iterate f y z \<Longrightarrow> f x = Some y \<Longrightarrow> iterate f x z"
-  by (induction f y z rule: iterate.induct) auto
+lemma iter_prestep: "iterate f y z \<Longrightarrow> f x = Some y \<Longrightarrow> iterate f x z"
+  by (induction f y z rule: iterate.induct) (simp_all add: iter_one)
 
 lemma [elim]: "iterate f x y \<Longrightarrow> iterate f y z \<Longrightarrow> iterate f x z"
   proof (induction f x y rule: iterate.induct)
   case iter_refl
     thus ?case by simp
   next case (iter_step f x y w)
-    hence "iterate f y z" by auto
+    with iter_prestep have "iterate f y z" by fast
     with iter_step show ?case by simp
   qed
 
